theories/small_step.v
@@ -1,0 +1,74 @@
+Require Import syntax.
+
+Definition is_value v :=
+    match v with
+    | Value _ => True
+    | Empty => True
+    | Conflict => True
+    | _ => False
+    end.
+
+Inductive sred: term -> term -> Prop :=
+  | sred_beta:
+    forall t u v,
+      t.[Value v/] = u ->
+      sred (App (Lam t) (Value v)) u
+  | sred_app_left:
+    forall t1 t2 u,
+      sred t1 t2 ->
+      sred (App t1 u) (App t2 u)
+  | sred_app_right:
+    forall t sigma u1 u2,
+      sred u1 u2 ->
+      sred (App (Value (Closure t sigma)) u1) (App (Value (Closure t sigma)) u2)
+
+  | sred_default_conflict:
+    forall ts ts1 ti ts2 tj ts3 tjust tcons,
+    List.Forall is_value ts ->
+    ti <> Empty ->
+    tj <> Empty ->
+    ts = (ts1 ++ ti::ts2++tj::ts3)%list ->
+    sred (Default ts tjust tcons) Conflict
+  | sred_DefaultEValue:
+    forall ts1 ti ts2 tjust tcons,
+    List.Forall (eq Empty) ts1 ->
+    List.Forall (eq Empty) ts2 ->
+    ti <> Empty ->
+    is_value ti ->
+    sred (Default (ts1++ti::ts2) tjust tcons) ti
+ | sred_DefaultE:
+    forall ts1 ti ti' ts2 tj tc,
+    sred ti ti' ->
+    (List.Forall is_value ts1) ->
+    sred (Default (ts1++ti::ts2) tj tc) (Default (ts1++ti'::ts2) tj tc)
+  | sred_DefaultJ:
+    forall ts tj1 tj2 tc,
+    List.Forall (eq Empty) ts ->
+    sred tj1 tj2 ->
+    sred (Default ts tj1 tc) (Default ts tj2 tc)
+  | sred_DefaultJTrue:
+    forall ts tc,
+    List.Forall (eq Empty) ts ->
+    sred (Default ts (Value (Bool true)) tc) tc
+  | sred_DefaultJFalse:
+    forall ts tc,
+    List.Forall (eq Empty) ts ->
+    sred (Default ts (Value (Bool false)) tc) Empty
+  | sred_DefaultJEmpty:
+    forall ts tc,
+    List.Forall (eq Empty) ts ->
+    sred (Default ts Empty tc) Empty
+  | sred_DefaultJConflict:
+    forall ts tc,
+    List.Forall (eq Empty) ts ->
+    sred (Default ts Conflict tc) Empty
+.
+
+
+Definition subst_of_env sigma :=
+  fun n =>
+  match List.nth_error sigma n with
+  | None => ids n
+  | Some t => Value t
+  end
+.
