theories/small_step_equivalence.v
@@ -1,0 +1,211 @@
+Require Import syntax continuations small_step sequences tactics.
+Import List.ListNotations.
+
+Definition subst_of_env sigma :=
+  fun n =>
+  match List.nth_error sigma n with
+  | None => ids (n - List.length sigma)
+  | Some t => Value t
+  end
+.
+
+Lemma subst_env_0: forall t v, t.[subst_of_env [v]] = t.[Value v/].
+Proof.
+  intros.
+  repeat f_equal.
+  eapply FunctionalExtensionality.functional_extensionality.
+  unfold subst_of_env.
+  induction x; simpl; eauto.
+  induction x; simpl; eauto.
+Qed.
+
+Definition apply_cont
+  (k: cont)
+  (param1: term * list value)
+  : term * list value :=
+  let '(t, sigma) := param1 in
+  match k with
+  | CAppR t2 =>
+    (App t t2.[subst_of_env sigma], sigma)
+  | CBinopL op v1 =>
+    (Binop op (Value v1) t, sigma)
+  | CBinopR op t2 =>
+    (Binop op t t2.[subst_of_env sigma], sigma)
+  | CClosure t_cl sigma_cl =>
+    (App (Value (Closure t_cl sigma_cl)) t, sigma)
+  | CReturn sigma' => (t, sigma')
+  | CDefault (Some v) ts tj tc =>
+    (Default (t::(Value v)::ts)..[subst_of_env sigma] tj.[subst_of_env sigma] tc.[subst_of_env sigma], sigma)
+  | CDefault None ts tj tc =>
+    (Default (t::ts)..[subst_of_env sigma] tj.[subst_of_env sigma] tc.[subst_of_env sigma], sigma)
+  | CDefaultBase tc =>
+    (Default nil t tc.[subst_of_env sigma], sigma)
+  | CMatch t1 t2 =>
+    (Match_ t t1.[subst_of_env sigma] t2.[up (subst_of_env sigma)], sigma)
+  | CSome =>
+    (ESome t, sigma)
+  end.
+
+Definition apply_conts
+  (kappa: list cont)
+  (t: term)
+  (sigma: list value): term * list value :=
+  List.fold_right apply_cont (t, sigma) kappa.
+
+Definition apply_return (r: result) :=
+  match r with
+  | RValue v => Value v
+  | REmpty => Empty
+  | RConflict => Conflict
+  end.
+
+Definition apply_state (s: state): term :=
+  match s with
+  | mode_eval t stack env =>
+    fst (apply_conts stack t env)
+  | mode_cont stack env r =>
+    fst (apply_conts stack (apply_return r) env)
+  end.
+
+
+Definition subst_cont
+  (k: cont)
+  (sigma: list value): cont :=
+  match k with
+  | CAppR t2 => CAppR t2.[subst_of_env sigma]
+  | CBinopL op v1 => CBinopL op v1
+  | CBinopR op t2 => CBinopR op t2.[subst_of_env sigma]
+  | CClosure t_cl sigma_cl => CClosure t_cl sigma_cl
+  | CReturn sigma' => CReturn sigma'
+  | CDefault (Some v) ts tj tc =>
+    CDefault
+      (Some v)
+      ts..[subst_of_env sigma]
+      tj.[subst_of_env sigma]
+      tc.[subst_of_env sigma]
+  | CDefault None ts tj tc =>
+    CDefault
+      None
+      ts..[subst_of_env sigma]
+      tj.[subst_of_env sigma]
+      tc.[subst_of_env sigma]
+  | CDefaultBase tc =>
+    CDefaultBase tc.[subst_of_env sigma]
+  | CMatch t1 t2 =>
+    CMatch t1.[subst_of_env sigma] t2.[up (subst_of_env sigma)]
+  | CSome => CSome
+  end
+.
+
+Fixpoint subst_conts
+  (kappa: list cont)
+  (sigma: list value): list cont :=
+  match kappa with
+  | (CReturn sigma) :: t =>
+    t
+  | h :: t =>
+    subst_cont h sigma :: subst_conts t sigma
+  | [] =>
+    []
+  end
+.
+
+Inductive equiv: state -> state -> Prop :=
+| EQ_trans:
+  forall s1 s2 s3,
+    equiv s1 s2 -> equiv s2 s3 -> equiv s1 s3
+| EQ_relf:
+  forall s1,
+     equiv s1 s1
+| EQ_sym:
+  forall s1 s2,
+    equiv s1 s2 -> equiv s2 s1
+| EQ_subst_env_eval:
+  forall t kappa env,
+    equiv
+      (mode_eval t kappa env)
+      (mode_eval t.[subst_of_env env] (subst_conts kappa env) [])
+| EQ_step:
+  forall s1 s2,
+    cred s1 s2 -> equiv s1 s2
+  (* forall t t' k kappa env,
+    cred (mode_eval t kappa env) (mode_eval t' (k::kappa) env) ->
+    equiv (mode_eval t kappa env) (mode_eval t' (k :: kappa) env) *)
+.
+
+Definition env s:=
+  match s with
+  | mode_eval _ _ sigma => sigma
+  | mode_cont _ sigma _ => sigma
+  end
+.
+
+Lemma equiv_append_stack:
+  forall s1 s2,
+  equiv s1 s2 ->
+  forall kappa,
+  equiv (append_stack s1 kappa) (append_stack s2 kappa).
+Proof.
+  intros s1 s2.
+  induction 1; intros.
+  { eapply EQ_trans; eauto. }
+  { eapply EQ_relf; eauto. }
+  { eapply EQ_sym; eauto. }
+  { simpl in *; subst. }
+  { eapply EQ_step.
+    eapply append_stack_stable; eauto.
+  }
+Admitted.
+
+Theorem sred_cred t1 t2 :
+  sred t1 t2 ->
+    exists s2,
+    star cred (mode_eval t1 [] []) s2 /\
+    equiv s2 (mode_eval t2 [] []).
+Proof.
+  induction 1.
+  {
+    eexists; split.
+    { repeat (eapply star_step; [solve [econstructor]|]).
+      eapply star_refl.
+    }
+    subst.
+    replace (t.[Value v/]) with (t.[subst_of_env [v]]).
+    replace ([]) with (subst_conts [CReturn []] [v]).
+    eapply EQ_subst_env_eval.
+    simpl; eauto.
+    eapply subst_env_0.
+  }
+  {
+    unpack.
+    eexists; split.
+    { repeat (eapply star_step; [solve [econstructor]|]).
+      rewrite append_stack_all_eval.
+      eapply append_stack_stable_star.
+      eauto.
+    }
+    { eapply EQ_trans. eapply equiv_append_stack. eauto. simpl.
+      eapply EQ_sym. eapply EQ_step. econstructor. }
+  }
+  {
+    unpack; eexists; split.
+    { repeat (eapply star_step; [solve [econstructor]|]).
+      rewrite append_stack_all_eval.
+      eapply append_stack_stable_star.
+      eauto.
+    }
+    { eapply EQ_trans. eapply equiv_append_stack. eauto. simpl.
+      eapply EQ_sym. eapply EQ_trans. eapply EQ_step.
+      econstructor.
+      eapply EQ_trans.
+      eapply EQ_step. econstructor.
+      eapply EQ_step. econstructor.
+    }
+  }
+  { (* DConflict case. *)
+    unpack; subst; eexists; split.
+    { repeat (eapply star_step; [solve [econstructor]|]). admit alain. }
+  }
+  { induction ti; simpl in *; tryfalse.
+
+  }
