theories/translation.v
@@ -1,0 +1,177 @@
+Require Import syntax.
+
+Inductive pure := Pure | Impure.
+
+Notation monad_bind t1 t2 := (Match_ t1 ENone t2).
+
+
+Fixpoint monad_handle_one (ts: list term) : term :=
+  match ts with
+  | nil => ESome (Var 0)
+  | cons thead ttail =>
+    Match_ (lift 1 thead)
+      (monad_handle_one ttail)
+      (Conflict)
+  end.
+
+Fixpoint monad_handle_zero ts tj tc: term :=
+  match ts with
+  | nil => monad_bind tj (App (App (App (Var 0) (Var 0)) (lift 1 tc)) ENone)
+  | cons thead ttail =>
+    Match_ thead
+      (monad_handle_zero ttail tj tc)
+      (monad_handle_one ttail)
+  end.
+
+
+
+Definition monad_handle ts tj tc: term :=
+  monad_handle_zero ts tj tc
+.
+
+Fixpoint trans (Delta: list pure) t { struct t } :=
+  match t with
+  | Var x =>
+    match List.nth_error Delta x with
+    | Some Impure => ESome (Var x)
+    | Some Pure => Var x
+    | None => Conflict
+    end
+  | Lam t =>
+    ESome (Lam (trans (Pure :: Delta) t))
+  | App (Lam body) arg => (* let arg in body *)
+    monad_bind (trans Delta arg) (trans (Pure :: Delta) body)
+  (* | D.App () =>
+    MBind (trans Delta arg) (ESome (L.EOp op) ) *)
+  | App (Var f) arg =>
+    match List.nth_error Delta f with
+    | Some b =>
+      if b then
+        (monad_bind (trans Delta arg)
+          (App (lift 1 (Var f)) (Var 0))
+        )
+      else
+        (monad_bind (Var f)
+          (monad_bind (lift 1 (trans Delta arg))
+            (App (lift 1 (Var 0)) (Var 0))
+          )
+        )
+    | None => Conflict
+    end
+  | Binop op e1 e2 =>
+    monad_bind (trans Delta e1)
+      (monad_bind (trans Delta e2)
+        (Binop op (Var 1) (Var 0))
+      )
+
+  (* | D.App f arg =>
+    monad_bind (trans Delta f) (monad_bind (lift 1 (trans Delta arg)) (L.App (lift 1 (L.Var 0)) (L.Var 0))) *)
+  | Default es ej ec =>
+    monad_handle
+      (List.map (trans Delta) es)
+      (trans Delta ej)
+      (trans Delta ec)
+  | Value v =>
+    ESome (Value v)
+  | Empty =>
+    ENone
+  (* incompatible *)
+  | Conflict => Conflict
+  | FreeVar _ => Conflict
+  | App _ _ => Conflict
+  | Match_ _ _ _ => Conflict
+  | ENone => Conflict
+  | ESome _ => Conflict
+  (* | D.BinOp op t1 t2 => L..ECompile*)
+  end.
+
+Require Import continuations.
+
+
+Definition subst_of_env sigma :=
+  fun n =>
+  match List.nth_error sigma n with
+  | None => ids n
+  | Some t => Value t
+  end
+.
+Search (?x = S ?x).
+
+Require Import tactics.
+Require Import sequences typing.
+
+Theorem correction_continuations:
+  forall s1 s2,
+  (exists GGamma Gamma T, jt_state GGamma Gamma s1 T) ->
+  cred s1 s2 ->
+  forall Delta,
+  exists target,
+    star cred
+      (mode_eval (trans Delta (apply_state s1)) nil nil) target /\
+    star cred
+      (mode_eval (trans Delta (apply_state s2)) nil nil) target.
+Proof.
+  intros s1 s2 [GGamma [Gamma [T Htyped]]] Hcred.
+  pose proof (cred_stack_lenght_at_most_one_precise _ _ Hcred);
+  simpl in *;
+  repeat match goal with
+    | [h: _ \/ _ |- _] => destruct h
+    | [h: False |- _] => destruct h
+    | [h: _ /\ _ |- _] => destruct h
+  end.
+  { induction Hcred; try solve [simpl in *; tryfalse (eapply n_Sn; eauto)].
+    6:{
+      induction kappa.
+      { simpl in *.
+        eexists; split.
+        { eapply star_step. econstructor.
+          eapply star_step. econstructor.
+          eapply star_step. econstructor.
+          eapply star_step. econstructor.
+          eapply star_step. econstructor.
+          eapply star_step. econstructor.
+          edestruct (typing.correct (mode_eval (trans Delta e2.[subst_of_env sigma]) nil (v :: nil))). { admit alain. }
+          eapply star_trans.
+          { rewrite append_stack_all_eval.
+            rewrite append_env_all_eval.
+            eapply append_stack_stable_star.
+            unpack. eauto.
+          }
+          unpack.
+          induction x; simpl in *; subst; try congruence; simpl.
+          assert (exists Delta Gamma T, jt_state Delta Gamma (mode_cont nil env result) (TOption T)). { admit alain. }
+          unpack.
+          induction result; repeat inv_jt.
+          { eapply star_step. econstructor.
+            eapply star_step. econstructor.
+            eapply star_step. econstructor.
+            eapply star_refl.
+          }
+          { eapply star_step. econstructor.
+            eapply star_step. econstructor.
+            eapply star_step.
+            eapply star_refl.
+          }
+
+            eapply H2.
+            eapply 
+
+
+      simpl monad_bind.
+
+
+      simpl.
+
+    }
+    all: admit alain.
+  }
+  { induction Hcred; simpl in *; tryfalse (eapply n_Sn; eauto).
+    all: admit alain.
+  }
+  { induction Hcred; simpl in *; tryfalse (eapply n_Sn; eauto).
+    all: admit alain.
+  }
+  { induction Hcred; simpl in *; tryfalse (eapply n_Sn; eauto).
+    all: admit alain.
+  }
+Admitted.
